Implement oracle_ok plan.

src/BlockAllocator.v
@@ -21,18 +21,18 @@ Fixpoint get_first_zero l :=
     end
   end.
 
-Definition upd {T} i l (v: T) := firstn (length l) (firstn i l ++ v::skipn (S i) l).
+Definition upd_list {T} i l (v: T) := firstn (length l) (firstn i l ++ v::skipn (S i) l).
 
 Theorem upd_valid_zero:
   forall i l,
     valid_bitlist l ->
-    valid_bitlist (upd i l 0).
+    valid_bitlist (upd_list i l 0).
 Proof. Admitted.
 
 Theorem upd_valid_one:
   forall i l,
     valid_bitlist l ->
-    valid_bitlist (upd i l 1).
+    valid_bitlist (upd_list i l 1).
 Proof. Admitted.
 
 Axiom value_to_bits: value -> bitlist.
@@ -41,12 +41,26 @@ Axiom value_to_bits_to_value : forall v, bits_to_value (value_to_bits v) = v.
 Axiom bits_to_value_to_bits : forall l, value_to_bits (bits_to_value l) = l.                                                                   
 Open Scope pred_scope.
 
+Fixpoint ptsto_bits' (dh: disk value) bits n : @pred addr addr_dec (set value) :=
+  match bits with
+  | nil => emp
+  | b::l =>
+    (exists vs,
+    (S n) |-> vs *
+    match b with
+    | 0 => [[ dh n = None ]]
+    | 1 => [[ dh n = Some (fst vs) ]]
+    | _ => [[ False ]]
+    end) *
+    ptsto_bits' dh l (S n)
+  end.
+      
+Definition ptsto_bits dh bits := ptsto_bits' dh bits 0.
+
 Definition rep (dh: disk value) : @pred addr addr_dec (set value) :=
-  fun d => (exists bitmap bl rest,
+  (exists bitmap bl,
     let bits := bits (value_to_bits bitmap) in
-    0 |-> (bitmap, bl) * rest *
-    [[forall i, nth i bits 0 = 0 -> dh i = None]] *
-    [[(forall i, nth i bits 0 = 1 -> exists vs, d (S i) = Some vs /\ dh i = Some (fst vs))%type]])%pred d.
+    0 |-> (bitmap, bl) * ptsto_bits dh bits)%pred.
 
 Definition alloc (v': value) : prog (option addr) :=
   v <- Read 0;
@@ -56,7 +70,7 @@ Definition alloc (v': value) : prog (option addr) :=
   
   if lt_dec index block_size then
     _ <- Write (S index) v';
-    _ <- Write 0 (bits_to_value (Build_bitlist (upd index bits 1) (upd_valid_one index bits valid)));
+    _ <- Write 0 (bits_to_value (Build_bitlist (upd_list index bits 1) (upd_valid_one index bits valid)));
     Ret (Some index)
   else
     Ret None.
@@ -91,17 +105,27 @@ Definition free a : prog unit :=
   let valid := valid (value_to_bits v) in
   if lt_dec a block_size then
     if addr_dec (nth a bits 0) 1 then
-      Write 0 (bits_to_value (Build_bitlist (upd a bits 0) (upd_valid_zero a bits valid)))
+      Write 0 (bits_to_value (Build_bitlist (upd_list a bits 0) (upd_valid_zero a bits valid)))
     else
       Ret tt
   else
     Ret tt.
 
-(*
+Lemma star_split:
+    forall (AT : Type) (AEQ : EqDec AT) (V : Type)
+      (p q : @pred AT AEQ V) (m : @mem AT AEQ V),
+      (p * q)%pred m ->
+      (exists m1 m2, mem_disjoint m1 m2 /\ p m1 /\ q m2 /\ mem_union m1 m2 = m)%type.
+  Proof.
+    intros; unfold sep_star in *; rewrite sep_star_is in *;
+      destruct H; cleanup; eauto.
+    do 2 eexists; intuition eauto.
+  Qed.
+
 Theorem hoare_triple_pre_ex':
   forall T V (p: prog T) pre post crash,
-  (forall (v: V), hoare_triple (fun a => pre v a) p post crash) ->
-  hoare_triple (fun a => exists (v: V), pre v a) p post crash.
+  (forall (v: V), hoare_triple (fun a d => pre v a d) p post crash) ->
+  hoare_triple (fun a d => (exists (v: V), pre v a) d) p post crash.
 Proof.
   unfold hoare_triple; intros.
   destruct_lift H0; cleanup.
@@ -109,16 +133,25 @@ Proof.
 Qed.
 
 Theorem hoare_triple_pre_ex:
-  forall T V (p: prog T) pre post crash F,
-  (forall (v: V), hoare_triple (fun a => F * pre v a) p post crash) ->
-  hoare_triple (fun a => F * exists (v: V), pre v a) p post crash.
+  forall T V (p: prog T) pre post crash F P,
+  (forall (v: V), hoare_triple (fun a d => ((F * (fun d' => pre v a d')) * [[ P a d ]]) d) p post crash) ->
+  hoare_triple (fun a d => ((F * (fun d' => (exists (v: V), pre v a) d')) * [[ P a d ]]) d) p post crash.
 Proof.
   intros.
   eapply hoare_triple_strengthen_pre.
   apply hoare_triple_pre_ex'.
-  instantiate (1:= fun v a => F * pre v a).
+  instantiate (1:= fun v a d => ((F * (pre v a)) * [[ P a d ]]) d).
   simpl; eauto.
-  intros; cancel.
+  intros; norm.
+  unfold stars; simpl.
+  intros mx Hmx; simpl in *.
+  destruct_lift Hmx.
+  destruct_lift H0.
+  destruct_lift H0.
+  exists dummy.
+  pred_apply' H0; norm.
+  cancel.
+  all: eauto.
 Qed.
 
 Lemma upd_eq':
@@ -134,7 +167,7 @@ Theorem alloc_ok:
   << o >>
    (rep dh)
    (alloc v)
-  << o', r >>
+  << r >>
    (exists dh',
     rep dh' *
      [[(r = None /\ dh' = dh) \/
@@ -144,198 +177,101 @@ Theorem alloc_ok:
      [[(dh' = dh) \/
        (exists h, dh' = upd dh h v)%type]]).
 Proof.
-  intros.
-  unfold alloc; simpl.
+  unfold alloc; intros dh v.
   unfold rep.
-  repeat (apply hoare_triple_pre_ex; intros).
-
-  eapply hoare_triple_pimpl;
-  try solve [intros; simpl in *; eauto].
-  eapply hoare_triple_strengthen_pre;
-  [apply read_okay | intros; simpl; cancel].
-
-  intros; simpl.
-  destruct (addr_dec (value_to_nat r) 0); simpl.
+  repeat (apply extract_exists; intros).
+  eapply crash_weaken.
+  eapply bind_ok.  
+  eapply pre_strengthen.
+  eapply add_frame.
+  apply read_ok.
+  cancel.
+  simpl; intros; cancel.
+ 
+  intros; destruct_lifts.
+  destruct (lt_dec (get_first_zero (bits (value_to_bits v0))) block_size); simpl in *.
   {
-    intros; simpl. 
-    eapply hoare_triple_pimpl;
-    try solve [intros; simpl in *; eauto].
-    eapply hoare_triple_strengthen_pre;
-      [apply write_okay | intros; simpl; cancel].
+    eapply hoare_triple_strengthen_pre.
+    eapply crash_weaken.
+    eapply bind_ok.
+    eapply add_frame.
+    apply write_ok.
 
-    intros; simpl.
-    destruct_pairs.
-    eapply hoare_triple_pimpl;
-    try solve [intros; simpl in *; eauto].
-    eapply hoare_triple_strengthen_pre;
-      [apply write_okay | intros; simpl; cancel].
-    {
-      intros; simpl.
-      eapply hoare_triple_strengthen_pre.
-      eapply hoare_triple_weaken_post_strong.
-      eapply hoare_triple_weaken_crash_strong.
-      apply ret_okay.  
-      3: intros; simpl; cancel.
+    simpl; intros; eauto.
+
+    simpl; intros.
+    eapply hoare_triple_strengthen_pre.
+    eapply crash_weaken.
+    eapply bind_ok.
+    eapply add_frame.
+    eapply write_ok.
+
+    simpl; intros; eauto.
+
+    simpl in *; intros.
+    eapply hoare_triple_strengthen_pre.
+    eapply crash_weaken.
+    eapply post_weaken.
+    eapply add_frame.
+    apply ret_ok.
+
+    - (* post *)
+      simpl; intros.
+      admit.
+    - eauto.
+    - simpl; intros.
+      cancel.
+      admit.
+    - eauto.
+    - simpl; intros; cancel.
+      norm; simpl. 
+      cancel.
       
-      intros; simpl;
-        norm; [cancel|].
-      eassign (upd dh 1 v).
-      rewrite nat_to_value_to_nat; eauto.
-      rewrite upd_eq'.
-      repeat rewrite upd_ne; eauto.
-      destruct_lift H;        
-        destruct_lift H0; cleanup.
-      intuition (eauto; try omega).
-      rewrite upd_ne; eauto.
-      omega.
-
-      intros; simpl.
-      norm; [cancel|].
-      eassign (upd dh 1 v).
-      rewrite nat_to_value_to_nat; eauto.
-      rewrite upd_eq'.
-      repeat rewrite upd_ne; eauto.
-      destruct_lift H;
-        destruct_lift H0; cleanup.
-      intuition (eauto; try omega).
-      rewrite upd_ne; eauto.
-      omega.
-    }
-    
-    all: intros; simpl in *;
-      destruct_lift H;
-      destruct_lift H0; cleanup;
-        cancel; eauto.
+      intros m Hm; simpl in *.
+      pred_apply; cancel.
+      admit.
+      destruct_lifts; cleanup.
+      do 2 eexists; intuition reflexivity.
+      
+      admit.
+      destruct_lifts; cleanup.
+      do 2 eexists; intuition reflexivity.
+      eauto.
+    - eauto.
+    - simpl; intros; cancel.
+      intros m Hm; simpl in *.
+      pred_apply; cancel.
+      admit.
+      destruct_lifts; cleanup.
+      do 2 eexists; intuition reflexivity.
+      
+      admit.
+      destruct_lifts; cleanup.
+      do 2 eexists; intuition reflexivity.
   }
-  destruct (addr_dec (value_to_nat r) 1); simpl.
   {
-    intros; simpl. 
-    eapply hoare_triple_pimpl;
-    try solve [intros; simpl in *; eauto].
-    eapply hoare_triple_strengthen_pre;
-      [apply write_okay | intros; simpl; cancel].
+    simpl in *; intros.
+    eapply hoare_triple_strengthen_pre.
+    eapply crash_weaken.
+    eapply post_weaken.
+    eapply add_frame.
+    apply ret_ok.
 
-    intros; simpl.
-    destruct_pairs.
-    eapply hoare_triple_pimpl;
-    try solve [intros; simpl in *; eauto].
-    eapply hoare_triple_strengthen_pre;
-    [apply write_okay | intros; simpl; cancel].
-
-    {
-      intros; simpl.
-      eapply hoare_triple_strengthen_pre.
-      eapply hoare_triple_weaken_post_strong.
-      eapply hoare_triple_weaken_crash_strong.
-      apply ret_okay.  
-      3: intros; simpl; cancel.
-      
-      intros; simpl;
-        norm; [cancel|].
-      eassign (upd dh 2 v).
-      rewrite nat_to_value_to_nat; eauto.
-      rewrite upd_eq'.
-      repeat rewrite upd_ne; eauto.
-      destruct_lift H;
-        destruct_lift H0; cleanup.
-      intuition (eauto; try omega).
-      rewrite upd_ne; eauto.
-      omega.
-
-      intros; simpl.
-      norm; [cancel|].
-      eassign (upd dh 2 v).
-      rewrite nat_to_value_to_nat; eauto.
-      rewrite upd_eq'.
-      repeat rewrite upd_ne; eauto.
-      destruct_lift H;
-        destruct_lift H0; cleanup.
-      intuition (eauto; try omega).
-      rewrite upd_ne; eauto.
-      omega.
-    }
-    all: try solve [
-      intros; simpl in *;
-      destruct_lift H;
-        destruct_lift H0; cleanup;
-      cancel; eauto].      
+    - simpl; cancel.
+    - simpl; cancel.
+    - simpl; cancel.
+      cancel.
   }
-  destruct (addr_dec (value_to_nat r) 2); simpl.
   {
-    intros; simpl. 
-    eapply hoare_triple_pimpl;
-    try solve [intros; simpl in *; eauto].
-    eapply hoare_triple_strengthen_pre;
-    [apply write_okay | intros; simpl; cancel].
-    
-    intros; simpl.
-    destruct_pairs.
-    eapply hoare_triple_pimpl;
-    try solve [intros; simpl in *; eauto].
-    eapply hoare_triple_strengthen_pre;
-    [apply write_okay | intros; simpl; cancel].
-
-    {
-      intros; simpl.
-      eapply hoare_triple_strengthen_pre.
-      eapply hoare_triple_weaken_post_strong.
-      eapply hoare_triple_weaken_crash_strong.
-      apply ret_okay.  
-      3: intros; simpl; cancel.
-      
-      intros; simpl;
-        norm; [cancel|].
-      eassign (upd dh 1 v).
-      rewrite nat_to_value_to_nat; eauto.
-      rewrite upd_eq'.
-      repeat rewrite upd_ne; eauto.
-      destruct_lift H;
-        destruct_lift H0; cleanup.
-      intuition (eauto; try omega).
-      rewrite upd_ne; eauto.
-      omega.
-
-      intros; simpl.
-      norm; [cancel|].
-      eassign (upd dh 1 v).
-      rewrite nat_to_value_to_nat; eauto.
-      rewrite upd_eq'.
-      repeat rewrite upd_ne; eauto.
-      destruct_lift H;
-        destruct_lift H0; cleanup.
-      intuition (eauto; try omega).
-      rewrite upd_ne; eauto.
-      omega.
-    }
-    all: try solve [
-      intros; simpl in *;
-      destruct_lift H;
-        destruct_lift H0; cleanup;
-        norm; [cancel| intuition (eauto; try omega)]
-      ].
+    simpl; cancel.
+    admit.
   }
+  Unshelve.
+  all: eauto.
+  all: try econstructor; eauto.
+  exact emp.
+Admitted.
 
-  {
-      intros; simpl.
-      eapply hoare_triple_strengthen_pre.
-      eapply hoare_triple_weaken_post_strong.
-      eapply hoare_triple_weaken_crash_strong.
-      apply ret_okay.
-      3: intros; simpl; rewrite emp_star_r; eauto.
-      
-      intros; simpl; destruct_lift H; cleanup.
-      norm; [cancel| intuition (eauto; try omega)].
-
-      intros; simpl; destruct_lift H; cleanup.
-      norm; [cancel| intuition (eauto; try omega)].
-  }
-
-  all: try solve [
-       intros; simpl; destruct_lift H; cleanup;
-       norm; [cancel| intuition (eauto; try omega)]
-           ].
-Qed.
-*)
 Theorem read_ok:
   forall a dh,
   << o >>
@@ -343,10 +279,9 @@ Theorem read_ok:
    (read a)
   << r >>
   (rep dh *
-   [[ ~In Crash o ]] *
    [[(r = None /\ (dh a = None \/ a >= block_size)) \/
      (exists v, r = Some v /\ dh a = Some v)%type]])
-   (rep dh * [[ In Crash o ]]).
+   (rep dh).
 Proof. Admitted. (*
   intros.
   unfold read; simpl.
