src/Layer1.v
@@ -10,6 +10,7 @@ Section Layer1.
   | Cont : token.
 
   Definition token_dec : forall (t t': token), {t=t'}+{t<>t'}. decide equality. Defined.
+  Definition oracle := list token.
 
   Definition state := disk (set value).
   
@@ -20,7 +21,7 @@ Section Layer1.
   | Bind : forall T T', prog T -> (T -> prog T') -> prog T'.
    
   Inductive exec :
-    forall T, oracle token ->  state -> prog T -> @Result state T -> Prop :=
+    forall T, oracle ->  state -> prog T -> @Result state T -> Prop :=
   | ExecRead : 
       forall d a v,
         read d a = Some v ->
@@ -53,12 +54,55 @@ Section Layer1.
         exec o1 d1 p1 (Crashed d1') ->
         exec o1 d1 (Bind p1 p2) (Crashed d1')
 
+  | ExecReadFail : 
+      forall d a,
+        read d a = None ->
+        exec [Cont] d (Read a) (Failed d)
+             
+  | ExecWriteFail :
+      forall d a v,
+        read d a = None ->
+        exec [Cont] d (Write a v) (Failed d)
+
   | ExecBindFail :
       forall T T' (p1: prog T) (p2: T -> prog T')
         o st st1,
         exec o st p1 (Failed st1) ->
         exec o st (Bind p1 p2) (Failed st1).
-  (* TODO: add Failed cases *)
+
+  Fixpoint oracle_ok {T} (p: prog T) o s :=
+    match p with
+    | Bind p1 p2 =>
+      exists o1 o2,
+      o = o1++o2 /\
+      oracle_ok p1 o1 s /\
+      (forall s' r,
+          exec o1 s p1 (Finished s' r) ->
+          oracle_ok (p2 r) o2 s') /\
+      (forall s',
+          exec o1 s p1 (Crashed s') ->
+          o2 = []) /\
+      (forall s',
+          exec o1 s p1 (Failed s') ->
+          o2 = [])
+    | _ =>
+      o = [Cont] \/ o = [Crash]
+    end.
+
+  (*
+  Variable op : Type -> Type.
+  Inductive prog' : Type -> Type :=
+  | Ret' : forall T, T -> prog' T
+  | Bind' : forall T T', op T -> (T -> prog' T') -> prog' T'.
+
+  Fixpoint bind {T1} (p1 : prog' T1): forall T2, (T1 -> prog' T2) -> prog' T2 :=
+    match p1 with
+    | Ret' x =>
+      fun T p2 => p2 x
+    | Bind' o px =>
+      fun T p2 => Bind' o (fun x => bind (px x) p2)
+    end.
+   *)
   
 End Layer1.
 
