src/OpSpec.v
@@ -2,10 +2,10 @@ Require Import List BaseTypes Memx Predx.
 Require Import CommonAutomation SepAuto Layer1 ProgAuto HoareL1.
 Open Scope pred_scope.
 
-Theorem read_okay:
-  forall a v t,
+Theorem read_ok:
+  forall a v,
     << o >>
-     (a |-> v * [[ o = t::nil ]])
+     (a |-> v)
      (Read a)
     << r >>
      (a |-> v * [[r = fst v]])
@@ -14,24 +14,22 @@ Proof.
   intros.
   unfold hoare_triple; intros.
   destruct_lift H; subst.
-  destruct t; eexists;
+  eapply ptsto_valid' in H as Hx;
+    cleanup; eauto.  
+  split_ors; eexists;
     intuition eauto;
   econstructor; intuition eauto.
-  inversion H0.
-  unfold Disk.read in *;
-    eapply ptsto_valid' in H as Hx;
-    cleanup; eauto.  
+  unfold Disk.read in *; cleanup; eauto.
+  
   do 2 eexists; split; eauto.
-  unfold Disk.read in *;
-    eapply ptsto_valid' in H as Hx;
-    cleanup; eauto.  
   simpl in *; pred_apply; cancel; eauto.
+  inversion H0.
 Qed.
 
-Theorem write_okay:
-  forall a v v' t,
+Theorem write_ok:
+  forall a v v',
     << o >>
-     (a |-> v * [[ o = t::nil ]])
+     (a |-> v)
      (Write a v')
     << r >>
      (a |-> (v', (fst v::snd v)))
@@ -40,28 +38,25 @@ Proof.
   intros.
   unfold hoare_triple; intros.
   destruct_lift H; subst.
-  destruct t; eexists;
+  eapply ptsto_valid' in H as Hx;
+    cleanup; eauto.  
+  split_ors; eexists;
     intuition eauto;
     econstructor; intuition eauto.
-  inversion H0.
   
     unfold Disk.read in *;
-    eapply ptsto_valid' in H as Hx;
     cleanup; eauto.  
     do 2 eexists; split; eauto.
-    unfold Disk.read in *;
-    eapply ptsto_valid' in H as Hx;
-    cleanup; eauto.  
     unfold Disk.write; cleanup.
     unfold Disk.upd_disk.
-    eapply ptsto_upd'.
-    pred_apply; cancel; eauto.
+    eapply ptsto_upd'; eauto.
+    inversion H0.
 Qed.
 
-Theorem ret_okay:
-  forall T (v: T) t,
+Theorem ret_ok:
+  forall T (v: T),
     << o >>
-     (emp * [[ o = t::nil ]])
+     emp
      (Ret v)
     << r >>
      (emp * [[r = v]])
@@ -70,15 +65,16 @@ Proof.
   intros.
   unfold hoare_triple; intros.
   destruct_lift H; subst.
-  destruct t; eexists;
+  split_ors; eexists;
     intuition eauto.
-    econstructor; intuition eauto.
-    inversion H0.
-    simpl in *; cleanup; right; eexists; intuition eauto.
-    pred_apply; cancel.
+  
+  left; do 2 eexists; split; eauto.
+  pred_apply; cancel; eauto.
 
-    left.
-    do 2 eexists; split; eauto.
-    pred_apply; cancel; eauto.
+  econstructor; intuition eauto.
+  inversion H0.
+  
+  simpl in *; cleanup; right; eexists; intuition eauto.
+  pred_apply; cancel.    
 Qed.
 
